concurrency/Modular/bst.v
@@ -10,9 +10,9 @@ Module Info.
   Definition build_number := "".
   Definition build_tag := "".
   Definition build_branch := "".
-  Definition arch := "x86".
-  Definition model := "64".
-  Definition abi := "macos".
+  Definition arch := "aarch64".
+  Definition model := "default".
+  Definition abi := "apple".
   Definition bitsize := 64.
   Definition big_endian := false.
   Definition source_file := "bst.c".
@@ -26,6 +26,9 @@ Definition ___builtin_bswap : ident := $"__builtin_bswap".
 Definition ___builtin_bswap16 : ident := $"__builtin_bswap16".
 Definition ___builtin_bswap32 : ident := $"__builtin_bswap32".
 Definition ___builtin_bswap64 : ident := $"__builtin_bswap64".
+Definition ___builtin_cls : ident := $"__builtin_cls".
+Definition ___builtin_clsl : ident := $"__builtin_clsl".
+Definition ___builtin_clsll : ident := $"__builtin_clsll".
 Definition ___builtin_clz : ident := $"__builtin_clz".
 Definition ___builtin_clzl : ident := $"__builtin_clzl".
 Definition ___builtin_clzll : ident := $"__builtin_clzll".
@@ -36,6 +39,7 @@ Definition ___builtin_debug : ident := $"__builtin_debug".
 Definition ___builtin_expect : ident := $"__builtin_expect".
 Definition ___builtin_fabs : ident := $"__builtin_fabs".
 Definition ___builtin_fabsf : ident := $"__builtin_fabsf".
+Definition ___builtin_fence : ident := $"__builtin_fence".
 Definition ___builtin_fmadd : ident := $"__builtin_fmadd".
 Definition ___builtin_fmax : ident := $"__builtin_fmax".
 Definition ___builtin_fmin : ident := $"__builtin_fmin".
@@ -45,8 +49,6 @@ Definition ___builtin_fnmsub : ident := $"__builtin_fnmsub".
 Definition ___builtin_fsqrt : ident := $"__builtin_fsqrt".
 Definition ___builtin_membar : ident := $"__builtin_membar".
 Definition ___builtin_memcpy_aligned : ident := $"__builtin_memcpy_aligned".
-Definition ___builtin_read16_reversed : ident := $"__builtin_read16_reversed".
-Definition ___builtin_read32_reversed : ident := $"__builtin_read32_reversed".
 Definition ___builtin_sel : ident := $"__builtin_sel".
 Definition ___builtin_sqrt : ident := $"__builtin_sqrt".
 Definition ___builtin_unreachable : ident := $"__builtin_unreachable".
@@ -54,8 +56,6 @@ Definition ___builtin_va_arg : ident := $"__builtin_va_arg".
 Definition ___builtin_va_copy : ident := $"__builtin_va_copy".
 Definition ___builtin_va_end : ident := $"__builtin_va_end".
 Definition ___builtin_va_start : ident := $"__builtin_va_start".
-Definition ___builtin_write16_reversed : ident := $"__builtin_write16_reversed".
-Definition ___builtin_write32_reversed : ident := $"__builtin_write32_reversed".
 Definition ___compcert_i64_dtos : ident := $"__compcert_i64_dtos".
 Definition ___compcert_i64_dtou : ident := $"__compcert_i64_dtou".
 Definition ___compcert_i64_sar : ident := $"__compcert_i64_sar".
@@ -84,6 +84,7 @@ Definition _free : ident := $"free".
 Definition _freeDS : ident := $"freeDS".
 Definition _freelock2 : ident := $"freelock2".
 Definition _getValue : ident := $"getValue".
+Definition _inRange : ident := $"inRange".
 Definition _insertOp : ident := $"insertOp".
 Definition _key : ident := $"key".
 Definition _l : ident := $"l".
@@ -99,12 +100,15 @@ Definition _min : ident := $"min".
 Definition _n : ident := $"n".
 Definition _n_tree : ident := $"n_tree".
 Definition _node : ident := $"node".
+Definition _node_t : ident := $"node_t".
 Definition _p : ident := $"p".
 Definition _p1 : ident := $"p1".
 Definition _p2 : ident := $"p2".
 Definition _p_tree : ident := $"p_tree".
 Definition _pa : ident := $"pa".
 Definition _pb : ident := $"pb".
+Definition _pn : ident := $"pn".
+Definition _pn__2 : ident := $"pn__2".
 Definition _printDS : ident := $"printDS".
 Definition _printf : ident := $"printf".
 Definition _release : ident := $"release".
@@ -115,6 +119,7 @@ Definition _t : ident := $"t".
 Definition _tgp : ident := $"tgp".
 Definition _tgt : ident := $"tgt".
 Definition _thread_lock : ident := $"thread_lock".
+Definition _traverse : ident := $"traverse".
 Definition _tree_t : ident := $"tree_t".
 Definition _value : ident := $"value".
 Definition _x : ident := $"x".
@@ -912,16 +917,22 @@ Definition global_definitions : list (ident * globdef fundef type) :=
                    (mksignature (AST.Tlong :: AST.Tlong :: nil) AST.Tlong
                      cc_default)) (Tcons tlong (Tcons tlong Tnil)) tlong
      cc_default)) ::
- (___builtin_fmax,
-   Gfun(External (EF_builtin "__builtin_fmax"
-                   (mksignature (AST.Tfloat :: AST.Tfloat :: nil) AST.Tfloat
-                     cc_default)) (Tcons tdouble (Tcons tdouble Tnil))
-     tdouble cc_default)) ::
- (___builtin_fmin,
-   Gfun(External (EF_builtin "__builtin_fmin"
-                   (mksignature (AST.Tfloat :: AST.Tfloat :: nil) AST.Tfloat
-                     cc_default)) (Tcons tdouble (Tcons tdouble Tnil))
-     tdouble cc_default)) ::
+ (___builtin_fence,
+   Gfun(External (EF_builtin "__builtin_fence"
+                   (mksignature nil AST.Tvoid cc_default)) Tnil tvoid
+     cc_default)) ::
+ (___builtin_cls,
+   Gfun(External (EF_builtin "__builtin_cls"
+                   (mksignature (AST.Tint :: nil) AST.Tint cc_default))
+     (Tcons tint Tnil) tint cc_default)) ::
+ (___builtin_clsl,
+   Gfun(External (EF_builtin "__builtin_clsl"
+                   (mksignature (AST.Tlong :: nil) AST.Tint cc_default))
+     (Tcons tlong Tnil) tint cc_default)) ::
+ (___builtin_clsll,
+   Gfun(External (EF_builtin "__builtin_clsll"
+                   (mksignature (AST.Tlong :: nil) AST.Tint cc_default))
+     (Tcons tlong Tnil) tint cc_default)) ::
  (___builtin_fmadd,
    Gfun(External (EF_builtin "__builtin_fmadd"
                    (mksignature
@@ -950,25 +961,16 @@ Definition global_definitions : list (ident * globdef fundef type) :=
                      AST.Tfloat cc_default))
      (Tcons tdouble (Tcons tdouble (Tcons tdouble Tnil))) tdouble
      cc_default)) ::
- (___builtin_read16_reversed,
-   Gfun(External (EF_builtin "__builtin_read16_reversed"
-                   (mksignature (AST.Tlong :: nil) AST.Tint16unsigned
-                     cc_default)) (Tcons (tptr tushort) Tnil) tushort
-     cc_default)) ::
- (___builtin_read32_reversed,
-   Gfun(External (EF_builtin "__builtin_read32_reversed"
-                   (mksignature (AST.Tlong :: nil) AST.Tint cc_default))
-     (Tcons (tptr tuint) Tnil) tuint cc_default)) ::
- (___builtin_write16_reversed,
-   Gfun(External (EF_builtin "__builtin_write16_reversed"
-                   (mksignature (AST.Tlong :: AST.Tint :: nil) AST.Tvoid
-                     cc_default)) (Tcons (tptr tushort) (Tcons tushort Tnil))
-     tvoid cc_default)) ::
- (___builtin_write32_reversed,
-   Gfun(External (EF_builtin "__builtin_write32_reversed"
-                   (mksignature (AST.Tlong :: AST.Tint :: nil) AST.Tvoid
-                     cc_default)) (Tcons (tptr tuint) (Tcons tuint Tnil))
-     tvoid cc_default)) ::
+ (___builtin_fmax,
+   Gfun(External (EF_builtin "__builtin_fmax"
+                   (mksignature (AST.Tfloat :: AST.Tfloat :: nil) AST.Tfloat
+                     cc_default)) (Tcons tdouble (Tcons tdouble Tnil))
+     tdouble cc_default)) ::
+ (___builtin_fmin,
+   Gfun(External (EF_builtin "__builtin_fmin"
+                   (mksignature (AST.Tfloat :: AST.Tfloat :: nil) AST.Tfloat
+                     cc_default)) (Tcons tdouble (Tcons tdouble Tnil))
+     tdouble cc_default)) ::
  (___builtin_debug,
    Gfun(External (EF_external "__builtin_debug"
                    (mksignature (AST.Tint :: nil) AST.Tvoid
@@ -1018,11 +1020,10 @@ Definition public_idents : list ident :=
 (_freeDS :: _printDS :: _Inorder :: _getValue :: _changeValue :: _insertOp ::
  _findNext :: _surely_malloc :: _thread_lock :: _freelock2 :: _release ::
  _acquire :: _makelock :: _exit :: _free :: _malloc :: _printf ::
- ___builtin_debug :: ___builtin_write32_reversed ::
- ___builtin_write16_reversed :: ___builtin_read32_reversed ::
- ___builtin_read16_reversed :: ___builtin_fnmsub :: ___builtin_fnmadd ::
- ___builtin_fmsub :: ___builtin_fmadd :: ___builtin_fmin ::
- ___builtin_fmax :: ___builtin_expect :: ___builtin_unreachable ::
+ ___builtin_debug :: ___builtin_fmin :: ___builtin_fmax ::
+ ___builtin_fnmsub :: ___builtin_fnmadd :: ___builtin_fmsub ::
+ ___builtin_fmadd :: ___builtin_clsll :: ___builtin_clsl :: ___builtin_cls ::
+ ___builtin_fence :: ___builtin_expect :: ___builtin_unreachable ::
  ___builtin_va_end :: ___builtin_va_copy :: ___builtin_va_arg ::
  ___builtin_va_start :: ___builtin_membar :: ___builtin_annot_intval ::
  ___builtin_annot :: ___builtin_sel :: ___builtin_memcpy_aligned ::
