concurrency/Modular/bst_inst.v
@@ -1,0 +1,55 @@
+Require Import VST.concurrency.conclib.
+Require Import VST.floyd.proofauto.
+Require Import VST.atomics.general_locks.
+Require Import Coq.Sets.Ensembles.
+Require Import bst.puretree.
+Require Import bst.bst.
+Require Import VST.atomics.verif_lock_atomic.
+Require Import VST.floyd.library.
+
+#[export] Instance CompSpecs : compspecs. make_compspecs prog. Defined.
+Definition Vprog : varspecs.  mk_varspecs prog. Defined.
+
+Definition t_struct_tree := Tstruct _node noattr.
+Definition t_struct_tree_t := Tstruct _tree_t noattr.
+Definition t_struct_node := Tstruct _node_t noattr.
+Definition t_struct_pn := Tstruct _pn noattr.
+
+Definition number2Z (x : number) : Z :=
+  match x with
+    | Finite_Integer y => y
+    | Neg_Infinity => Int.min_signed
+    | Pos_Infinity => Int.max_signed
+  end.
+
+#[export] Instance pointer_lock : Ghost := discrete_PCM (val * val * range).
+Definition ghost_info : Type := (key * val)%type.
+
+(* This allows the range to be outdated while the ghost_info may be present or absent. *)
+#[export] Instance node_ghost : Ghost := prod_PCM pointer_lock (exclusive_PCM (option ghost_info)).
+Notation node_info := (@G node_ghost).
+
+Definition in_tree (g: gname) (g1 : gname) (pn: val) (lock: val):=
+      ghost_snap (P := gmap_ghost (K := gname)(A := discrete_PCM (val * val)) )
+        ({[g1 := (pn, lock)]}) g.
+
+Lemma in_tree_duplicate g gin pn lock:
+  in_tree g gin pn lock |-- in_tree g gin pn lock * in_tree g gin pn lock.
+Proof. by rewrite - bi.persistent_sep_dup. Qed.
+
+Class NodeRep : Type := {
+  node_rep_R : val -> range -> option (option ghost_info) -> gname -> mpred
+  }.
+
+#[global]Instance my_specific_tree_rep : NodeRep := {
+  node_rep_R := fun tp r g_info g =>
+    EX (ga gb : gname), EX (x : Z), EX (v pa pb : val), EX (locka lockb : val),
+      !!(g_info = Some (Some (x, v)) /\ and (Z.le Int.min_signed x) (Z.le x Int.max_signed) /\
+       is_pointer_or_null pa /\ is_pointer_or_null locka /\
+       is_pointer_or_null pb /\ is_pointer_or_null lockb /\
+          (tc_val (tptr Tvoid) v) /\ key_in_range x r = true) &&
+       data_at Ews t_struct_tree ((Vint (Int.repr x)), (v, (pa, pb))) tp * 
+       malloc_token Ews t_struct_tree tp *
+       in_tree g ga pa locka * in_tree g gb pb lockb
+}.
+
